@prefix : <http://www.semanticweb.org/owl/owlapi/turtle#> .
@prefix qb: <http://purl.org/linked-data/cube#> .
@prefix owl: <http://www.w3.org/2002/07/owl#> .
@prefix rdf: <http://www.w3.org/1999/02/22-rdf-syntax-ns#> .
@prefix xml: <http://www.w3.org/XML/1998/namespace> .
@prefix xsd: <http://www.w3.org/2001/XMLSchema#> .
@prefix foaf: <http://xmlns.com/foaf/0.1/> .
@prefix qb4o: <http://purl.org/qb4olap/cubes#> .
@prefix rdfs: <http://www.w3.org/2000/01/rdf-schema#> .
@prefix skos: <http://www.w3.org/2004/02/skos/core#> .
@prefix void: <http://rdfs.org/ns/void#> .
@prefix scovo: <http://purl.org/NET/scovo#> .
@prefix dbpedia: <http://dbpedia.org/resource/> .
@prefix dcterms: <http://purl.org/dc/terms/> .
@base <http://purl.org/qb4olap/cubes> .

<http://purl.org/qb4olap/cubes> rdf:type owl:Ontology ;
                                
                                rdfs:label "The QB4OLAP cube vocabulary, an extension to QB" ;
                                
                                dcterms:created "2012-12-06"^^xsd:date ;
                                
                                dcterms:modified "2014-10-03"^^xsd:date ;
                                
                                dcterms:title "Vocabulary for publishing OLAP data cubes" ;
                                
                                rdfs:comment "This vocabulary allows to publish and operate with OLAP cubes in RDF" ;
                                
                                owl:versionInfo "0.1.1" ;
                                
                                owl:imports <http://purl.org/linked-data/cube> ;
                                
                                dcterms:license <http://www.opendatacommons.org/licenses/pddl/1.0/> ;
                                
                                dcterms:contributor [ ] ,
[ ] .


#################################################################
#
#    Object Properties
#
#################################################################


###  http://purl.org/qb4olap/cubes#aggregateFunction

qb4o:aggregateFunction rdf:type owl:ObjectProperty ;
                       
                       rdfs:label "aggregate function"@en ;
                       
                       rdfs:comment "An alternative to qb:componentProperty which makes explicit that the component is an aggregate function"@en ;
                       
                       rdfs:subPropertyOf qb:componentProperty ;
                       
                       rdfs:isDefinedBy <http://purl.org/qb4olap/cubes> ;
                       
                       rdfs:range qb4o:AggregateFunction .



###  http://purl.org/qb4olap/cubes#cardinality

qb4o:cardinality rdf:type owl:ObjectProperty ;
                 
                 rdfs:label "cardinality"@en ,
                            "cardinality constraint"@en ;
                 
                 rdfs:comment "An alternative to qb:componentProperty which allows to specify a cardinality constraint in fact-level relationship"@en ;
                 
                 rdfs:subPropertyOf qb:componentProperty ;
                 
                 rdfs:isDefinedBy <http://purl.org/qb4olap/cubes> ;
                 
                 rdfs:range qb4o:Cardinality .


###  http://purl.org/qb4olap/cubes#pcCardinality

qb4o:pcCardinality rdf:type owl:ObjectProperty ;
                 
                 rdfs:label "cardinality"@en ,
                            "cardinality constraint"@en ;
                 
                 rdfs:comment "A property which allows to specify a cardinality constraint in a parent-child relationship"@en ;
                                
                 rdfs:isDefinedBy <http://purl.org/qb4olap/cubes> ;
                 
                 rdfs:range qb4o:Cardinality ;
                 
                 rdfs:domain qb4o:HierarchyStep .
                 

###  http://purl.org/qb4olap/cubes#childLevel

qb4o:childLevel rdf:type owl:ObjectProperty ;
                
                rdfs:label "child level"@en ;
                
                rdfs:comment "Child level component of a HierarchyStep"@en ;
                
                rdfs:isDefinedBy <http://purl.org/qb4olap/cubes> ;
                
                rdfs:domain qb4o:HierarchyStep ;
                
                rdfs:range qb4o:LevelInHierarchy .



###  http://purl.org/qb4olap/cubes#hasHierarchy

qb4o:hasHierarchy rdf:type owl:ObjectProperty ;
                  
                  rdfs:label "set of hierarchies in a dimensoin"@en ;
                  
                  rdfs:comment "Indicates the hierarchies that compose the dimension"@en ;
                  
                  rdfs:domain qb:DimensionProperty ;
                  
                  rdfs:isDefinedBy <http://purl.org/qb4olap/cubes> ;
                  
                  rdfs:range qb4o:HierarchyProperty ;
                  
                  owl:inverseOf qb4o:inDimension .



###  http://purl.org/qb4olap/cubes#hasLevel

qb4o:hasLevel rdf:type owl:ObjectProperty ;
              
              rdfs:label "set of levels in hierarchy"@en ;
              
              rdfs:comment "Indicates the levels that compose the hierarchy"@en ;
              
              rdfs:isDefinedBy <http://purl.org/qb4olap/cubes> ;
              
              rdfs:domain qb4o:HierarchyProperty ;
              
              rdfs:range qb4o:LevelProperty .
              

###  http://purl.org/qb4olap/cubes#hasAttribute

qb4o:hasAttribute rdf:type owl:ObjectProperty ;
              
              rdfs:label "Level has attribute"@en ;
              
              rdfs:comment "Indicates the attributes in an level"@en ;
              
              rdfs:isDefinedBy <http://purl.org/qb4olap/cubes> ;
              
              rdfs:domain qb4o:LevelProperty ;
              
              rdfs:range qb4o:AttributeProperty . 
 
###  http://purl.org/qb4olap/cubes#hasID

qb4o:hasID rdf:type owl:ObjectProperty ;
              
              rdfs:label "Level has ID attribute"@en ;
              
              rdfs:comment "Indicates the attribute that identifies level members"@en ;
              
              rdfs:isDefinedBy <http://purl.org/qb4olap/cubes> ;
              
              rdfs:domain qb4o:LevelProperty ;
              
              rdfs:range qb4o:AttributeProperty .  


###  http://purl.org/qb4olap/cubes#hierarchyComponent

qb4o:hierarchyComponent rdf:type owl:ObjectProperty ;
                        
                        rdfs:label "level component"@en ;
                        
                        rdfs:comment "Indicates the hierarchy component of a pair (hierarchy,level) represented by a resource of type LevelInHierarchy"@en ;
                        
                        rdfs:isDefinedBy <http://purl.org/qb4olap/cubes> ;
                        
                        rdfs:range qb4o:HierarchyProperty ;
                        
                        rdfs:domain qb4o:LevelInHierarchy .



###  http://purl.org/qb4olap/cubes#inDimension

qb4o:inDimension rdf:type owl:ObjectProperty ;
                 
                 rdfs:label "hierarchy belongs to dimension"@en ;
                 
                 rdfs:comment "Indicates to which dimension the hierarchy belongs"@en ;
                 
                 rdfs:range qb:DimensionProperty ;
                 
                 rdfs:isDefinedBy <http://purl.org/qb4olap/cubes> ;
                 
                 rdfs:domain qb4o:HierarchyProperty .



###  http://purl.org/qb4olap/cubes#inLevel

qb4o:inLevel rdf:type owl:ObjectProperty ;
             
             rdfs:label "level member in level"@en ;
             
             rdfs:comment "Indicates to which level the level member belongs"@en ;
             
             rdfs:isDefinedBy <http://purl.org/qb4olap/cubes> ;
             
             rdfs:domain qb4o:LevelMember ;
             
             rdfs:range qb4o:LevelProperty .



###  http://purl.org/qb4olap/cubes#level

qb4o:level rdf:type owl:ObjectProperty ;
           
           rdfs:label "level"@en ;
           
           rdfs:comment "An alternative to qb:componentProperty which makes explicit that the component is a level"@en ;
           
           rdfs:subPropertyOf qb:componentProperty ;
           
           rdfs:isDefinedBy <http://purl.org/qb4olap/cubes> ;
           
           rdfs:range qb4o:LevelProperty .



###  http://purl.org/qb4olap/cubes#levelComponent

qb4o:levelComponent rdf:type owl:ObjectProperty ;
                    
                    rdfs:label "level component"@en ;
                    
                    rdfs:comment "Indicates the level component of a pair (hierarchy,level) represented by a resource of type LevelInHierarchy"@en ;
                    
                    rdfs:isDefinedBy <http://purl.org/qb4olap/cubes> ;
                    
                    rdfs:domain qb4o:LevelInHierarchy ;
                    
                    rdfs:range qb4o:LevelProperty .



###  http://purl.org/qb4olap/cubes#parentLevel

qb4o:parentLevel rdf:type owl:ObjectProperty ;
                 
                 rdfs:label "parent level"@en ;
                 
                 rdfs:comment "Parent level component of a HierarchyStep"@en ;
                 
                 rdfs:isDefinedBy <http://purl.org/qb4olap/cubes> ;
                 
                 rdfs:domain qb4o:HierarchyStep ;
                 
                 rdfs:range qb4o:LevelInHierarchy .





#################################################################
#
#    Data properties
#
#################################################################


###  http://purl.org/qb4olap/cubes#hasAllLevel

qb4o:hasAllLevel rdf:type owl:DatatypeProperty ;
                 
                 rdfs:label "hasAllLevel"@en ;
                 
                 rdfs:comment "Indicates if the \"All\" level should be included in the hierarchy"@en ;
                 
                 rdfs:isDefinedBy <http://purl.org/qb4olap/cubes> ;
                 
                 rdfs:domain qb4o:HierarchyProperty ;
                 
                 rdfs:range xsd:boolean .





#################################################################
#
#    Classes
#
#################################################################


###  http://purl.org/qb4olap/cubes#AggregateFunction

qb4o:AggregateFunction rdf:type owl:Class ;
                       
                       rdfs:label "Aggregate function"@en ;
                       
                       rdfs:subClassOf qb:ComponentProperty ;
                       
                       rdfs:comment "The class of components which represent aggregate functions that are applied to compute measure aggregate values"@en ;
                       
                       rdfs:isDefinedBy <http://purl.org/qb4olap/cubes> .



###  http://purl.org/qb4olap/cubes#Avg

qb4o:Avg rdf:type owl:Class ;
         
         rdfs:label "AVG"@en ;
         
         rdfs:subClassOf qb4o:AggregateFunction ;
         
         rdfs:comment "Returns the arithmetic mean of a set of numeric values."@en ;
         
         rdfs:isDefinedBy <http://purl.org/qb4olap/cubes> .



###  http://purl.org/qb4olap/cubes#Cardinality

qb4o:Cardinality rdf:type owl:Class ;
                 
                 rdfs:label "Cardinality"@en ;
                 
                 rdfs:comment "Abstract class that represents different cardinalities restrictions in the hierarchies"@en ;
                 
                 rdfs:isDefinedBy <http://purl.org/qb4olap/cubes> .



###  http://purl.org/qb4olap/cubes#Count

qb4o:Count rdf:type owl:Class ;
           
           rdfs:label "COUNT"@en ;
           
           rdfs:subClassOf qb4o:AggregateFunction ;
           
           rdfs:comment "Returns the number of elements in a set of elements (the cardinality of the set)."@en ;
           
           rdfs:isDefinedBy <http://purl.org/qb4olap/cubes> .



###  http://purl.org/qb4olap/cubes#HierarchyProperty

qb4o:HierarchyProperty rdf:type owl:Class ;
                       
                       rdfs:label "Hierarchy property"@en ;
                       
                       rdfs:subClassOf qb:ComponentProperty ;
                       
                       rdfs:comment "The class of components which represent the hierarchies of a dimension"@en ;
                       
                       rdfs:isDefinedBy <http://purl.org/qb4olap/cubes> .



###  http://purl.org/qb4olap/cubes#HierarchyStep

qb4o:HierarchyStep rdf:type owl:Class ;
                   
                   rdfs:label "hierarchy step"@en ;
                   
                   rdfs:comment "Class that represents the reification of the qb4o:inHierarchy object property"@en ;
                   
                   rdfs:isDefinedBy <http://purl.org/qb4olap/cubes> .



###  http://purl.org/qb4olap/cubes#LevelInHierarchy

qb4o:LevelInHierarchy rdf:type owl:Class ;
                      
                      rdfs:comment "A class that represents the reification of the property inHierarchy"@en ;
                      
                      rdfs:isDefinedBy <http://purl.org/qb4olap/cubes> .



###  http://purl.org/qb4olap/cubes#LevelMember

qb4o:LevelMember rdf:type owl:Class ;
                 
                 rdfs:label "Level member"@en ;
                 
                 rdfs:subClassOf skos:Concept ;
                 
                 rdfs:comment "The class of components which represent the members of a level"@en ;
                 
                 rdfs:isDefinedBy <http://purl.org/qb4olap/cubes> .



###  http://purl.org/qb4olap/cubes#LevelProperty

qb4o:LevelProperty rdf:type owl:Class ;
                   
                   rdfs:label "Level property"@en ;
                   
                   rdfs:subClassOf qb:ComponentProperty ;
                   
                   rdfs:comment "The class of components which represent the levels of a hierarchy"@en ;
                   
                   rdfs:isDefinedBy <http://purl.org/qb4olap/cubes> .



###  http://purl.org/qb4olap/cubes#ManyToMany

qb4o:ManyToMany rdf:type owl:Class ;
                
                rdfs:label "N-M cardinality"@en ;
                
                rdfs:subClassOf qb4o:Cardinality ;
                
                rdfs:comment "Represents N-M cardinality constraint"@en ;
                
                rdfs:isDefinedBy <http://purl.org/qb4olap/cubes> .



###  http://purl.org/qb4olap/cubes#ManyToOne

qb4o:ManyToOne rdf:type owl:Class ;
               
               rdfs:label "N-1 cardinality"@en ;
               
               rdfs:subClassOf qb4o:Cardinality ;
               
               rdfs:comment "Represents N-1 cardinality constraint"@en ;
               
               rdfs:isDefinedBy <http://purl.org/qb4olap/cubes> .



###  http://purl.org/qb4olap/cubes#Max

qb4o:Max rdf:type owl:Class ;
         
         rdfs:label "MAX"@en ;
         
         rdfs:subClassOf qb4o:AggregateFunction ;
         
         rdfs:comment "Returns the maximum element in a set of elements, where a partial order is defined."@en ;
         
         rdfs:isDefinedBy <http://purl.org/qb4olap/cubes> .



###  http://purl.org/qb4olap/cubes#Min

qb4o:Min rdf:type owl:Class ;
         
         rdfs:label "MIN"@en ;
         
         rdfs:subClassOf qb4o:AggregateFunction ;
         
         rdfs:comment "Returns the minimum element in a set of elements, where a partial order is defined."@en ;
         
         rdfs:isDefinedBy <http://purl.org/qb4olap/cubes> .



###  http://purl.org/qb4olap/cubes#OneToMany

qb4o:OneToMany rdf:type owl:Class ;
               
               rdfs:label "1-N cardinality"@en ;
               
               rdfs:subClassOf qb4o:Cardinality ;
               
               rdfs:comment "Represents 1-N cardinality constraint"@en ;
               
               rdfs:isDefinedBy <http://purl.org/qb4olap/cubes> .



###  http://purl.org/qb4olap/cubes#OneToOne

qb4o:OneToOne rdf:type owl:Class ;
              
              rdfs:label "1_1 cardinality"@en ;
              
              rdfs:subClassOf qb4o:Cardinality ;
              
              rdfs:comment "Represents 1-1 cardinality constraint"@en ;
              
              rdfs:isDefinedBy <http://purl.org/qb4olap/cubes> .



###  http://purl.org/qb4olap/cubes#Sum

qb4o:Sum rdf:type owl:Class ;
         
         rdfs:label "SUM"@en ;
         
         rdfs:subClassOf qb4o:AggregateFunction ;
         
         rdfs:comment "Returns the numeric value obtained by adding a set of numeric values."@en ;
         
         rdfs:isDefinedBy <http://purl.org/qb4olap/cubes> .





#################################################################
#
#    Individuals
#
#################################################################


###  http://dbpedia.org/resource/Average

dbpedia:Average rdf:type owl:NamedIndividual ;
                
                owl:sameAs qb4o:Avg .



###  http://dbpedia.org/resource/Counting

dbpedia:Counting rdf:type owl:NamedIndividual ;
                 
                 owl:sameAs qb4o:Count .



###  http://dbpedia.org/resource/Max

dbpedia:Max rdf:type owl:NamedIndividual ;
            
            owl:sameAs qb4o:Max .



###  http://dbpedia.org/resource/Min

dbpedia:Min rdf:type owl:NamedIndividual ;
            
            owl:sameAs qb4o:Min .



###  http://dbpedia.org/resource/Summation

dbpedia:Summation rdf:type owl:NamedIndividual ;
                  
                  owl:sameAs qb4o:Sum .



###  http://purl.org/qb4olap/cubes#Avg

qb4o:Avg rdf:type qb4o:AggregateFunction ,
                  owl:NamedIndividual .



###  http://purl.org/qb4olap/cubes#Count

qb4o:Count rdf:type owl:NamedIndividual .



###  http://purl.org/qb4olap/cubes#Max

qb4o:Max rdf:type owl:NamedIndividual .



###  http://purl.org/qb4olap/cubes#Min

qb4o:Min rdf:type owl:NamedIndividual .



###  http://purl.org/qb4olap/cubes#Sum

qb4o:Sum rdf:type owl:NamedIndividual .




###  Generated by the OWL API (version 3.4.2) http://owlapi.sourceforge.net

